ulib/FStar.Monotonic.RRef.fst
@@ -1,8 +1,13 @@
 module FStar.Monotonic.RRef
 
 open FStar
-open FStar.ST
 open FStar.HyperHeap
+
+open FStar.HyperStack
+open FStar.HST
+
+module HS = FStar.HyperStack
+module HST = FStar.HST
 
 let reln (a:Type) = a -> a -> Type
 
@@ -10,7 +15,10 @@ let monotonic (a:Type) (b:reln a) =
   (forall x. b x x)                             (* reflexive *)
   /\ (forall x y z. b x y /\ b y z ==> b x z)   (* transitive *)
 
-abstract type m_rref (r:rid) (a:Type) (b:reln a) = rref r a
+//adding eternal region for now, since it is used with ralloc
+type rid = r:rid{HS.is_eternal_region r}
+
+abstract type m_rref (r:rid) (a:Type) (b:reln a) = x:HS.ref a{x.id = r}
 
 let haseq_m_rref (r:rid) (a:Type) (b:reln a) 
     : Lemma (requires True)
@@ -19,7 +27,10 @@ let haseq_m_rref (r:rid) (a:Type) (b:reln a)
     = ()
 
 val as_rref: #r:rid -> #a:Type -> #b:reln a -> m_rref r a b -> GTot (rref r a)
-let as_rref #r #a #b x = x
+let as_rref #r #a #b x = x.ref
+
+val as_reference: #r:rid -> #a:Type -> #b:reln a -> m_rref r a b  -> GTot (ref a)
+let as_reference #r #a #b x = x
 
 val m_contains : #r:rid -> #a:Type -> #b:reln a -> mr:m_rref r a b -> m:t -> GTot bool
 let m_contains #r #a #b mr m = HyperHeap.contains_ref (as_rref mr) m
@@ -39,16 +50,16 @@ val m_alloc: #a:Type
             -> init:a
             -> ST (m_rref r a b)
 		(requires (fun _ -> monotonic a b))
-		(ensures (fun h0 (m:m_rref r a b) h1 -> ralloc_post r init h0 (as_rref m) h1))
-let m_alloc #a #b r init = ST.ralloc r init
+		(ensures (fun h0 (m:m_rref r a b) h1 -> ralloc_post r init h0 (as_reference m) h1))
+let m_alloc #a #b r init = ralloc r init
 
 val m_read:#r:rid 
        -> #a:Type
        -> #b:reln a
        -> x:m_rref r a b
        -> ST a
-            (requires (fun h -> True))
-            (ensures (deref_post (as_rref x)))
+            (requires (fun h -> h `contains` (as_reference x)))
+            (ensures (deref_post (as_reference x)))
 let m_read #r #a #b x = !x
 
 val m_write:#r:rid 
@@ -57,8 +68,8 @@ val m_write:#r:rid
         -> x:m_rref r a b
         -> v:a
         -> ST unit
-              (requires (fun h0 -> b (m_sel h0 x) v))
-              (ensures (assign_post (as_rref x) v))
+              (requires (fun h0 -> h0 `contains` (as_reference x) /\ b (m_sel h0.h x) v))
+              (ensures (assign_post (as_reference x) v))
 let m_write #r #a #b x v = x := v
 
 inline type stable_on_t (#i:rid) (#a:Type) (#b:reln a) (r:m_rref i a b) (p:(t -> GTot Type0)) =
@@ -71,7 +82,7 @@ val witness: #r:rid
           -> m:m_rref r a b
           -> p:(t -> GTot Type0)
           -> ST unit
-                (requires (fun h0 -> p h0 /\ stable_on_t m p))
+                (requires (fun h0 -> p h0.h /\ stable_on_t m p))
                 (ensures (fun h0 _ h1 -> h0==h1 /\ witnessed p))
 let witness #r #a #b m p = ()
 
@@ -83,7 +94,7 @@ assume val weaken_witness : p:(t -> GTot Type0)
 val testify: p:(t -> GTot Type0)
           -> ST unit
                (requires (fun _ ->  witnessed p))
-               (ensures (fun h0 _ h1 -> h0==h1 /\ p h1))
+               (ensures (fun h0 _ h1 -> h0==h1 /\ p h1.h))
 let testify p = admit() //intentionally admitted
 
 
@@ -91,7 +102,7 @@ val testify_forall: #a:Type -> #p:(a -> t -> Type0)
        -> $s:squash (forall (x:a). witnessed (p x)) 
        -> ST unit
   (requires (fun h -> True))
-  (ensures (fun h0 _ h1 -> h0==h1 /\ (forall (x:a). p x h1)))
+  (ensures (fun h0 _ h1 -> h0==h1 /\ (forall (x:a). p x h1.h)))
 let testify_forall #a #p $s = admit() //intentionally admitted
 
 
@@ -99,8 +110,8 @@ val m_recall: #r:rid -> #a:Type -> #b:reln a
             -> m:m_rref r a b
 	    -> ST unit 
 	      (requires (fun h -> True))
-	      (ensures (fun h0 _ h1 -> h0==h1 /\ m_contains m h1))
-let m_recall #r #a #b m = FStar.ST.recall m
+	      (ensures (fun h0 _ h1 -> h0==h1 /\ h1 `contains` (as_reference m)))
+let m_recall #r #a #b m = recall m
 
 
 let rid_exists (r:rid) (h:t) = b2t(Map.contains h r)
